src/typechecker/FStarC.TypeChecker.Normalize.fst
@@ -47,6 +47,7 @@ module EMB = FStarC.Syntax.Embeddings
 module TcComm = FStarC.TypeChecker.Common
 module TEQ = FStarC.TypeChecker.TermEqAndSimplify
 module PO = FStarC.TypeChecker.Primops
+module Print = FStarC.Syntax.Print //bring into scope for show instances
 open FStarC.TypeChecker.Normalize.Unfolding
 
 (* Max number of warnings to print in a single run.
